changed sum type to inductive

LeanCourse/Memory.lean
@@ -6,7 +6,11 @@ structure IdT (β γ δ : Type) where
   pId  : δ
   flds : List (β ⊕ γ)
 
-def ValT α β γ δ := α ⊕ IdT β γ δ
+inductive ValT (α β γ δ : Type) where
+  | val (val : α)
+  | id  (id : IdT β γ δ)
+
+-- def ValT α β γ δ := α ⊕ IdT β γ δ
 
 open Sum
 
@@ -27,11 +31,11 @@ namespace Memory
 
 @[simp] def read [DecidableEq β] [DecidableEq γ] [DecidableEq δ] [Inhabited α] (mem : Memory α β γ δ) (id : IdT β γ δ) (fld : β ⊕ γ) : ValT α β γ δ :=
   match mem, id with
-  | .mtm, _ => inl default
+  | .mtm, _ => .val default
   | .write mem idM fldM val, _ => if idM = id && fldM = fld then val else read mem id fld
   | .add mem pId, ⟨idd, ids⟩ => if pId = idd
     then (match fld with
-      | inl _ => inl default
-      | inr _ => inr ⟨idd, fld :: ids⟩
+      | inl _ => .val default
+      | inr _ => .id ⟨idd, fld :: ids⟩
       )
     else read mem id fld
